checker/coq/linear.v
@@ -69,7 +69,7 @@ Qed.
 
 Definition eval_lincon lincon (theta : asg) :=
   (eval_linsum (fst lincon) theta) <= (snd lincon).
-  
+
 Definition check_lincon (lincon : lin_leq) (cl : clause) : bool :=
   negb (satb_lb (fst (linsum_db_from_negclause (fst lincon) cl)) (snd lincon)).
 
@@ -99,135 +99,17 @@ Definition check_linear_bnd (x : lin_leq) (bs : list (ivar*Z*Z)) (cl : clause) :
   check (BoundedConstraint LinearCon) (BoundedChecker LinearCon CheckLinear) (bs, x) cl.
 
 (* Computing solutions. *)
-Definition eval_linterm_zsol term zs :=
-  match zsol_val zs (snd term) with
-  | None => None
-  | Some x => Some ((fst term)*x)
-  end.
+Definition check_lincon_sol lincon theta :=
+  Z_leb (eval_linsum (fst lincon) theta) (snd lincon).
 
-Fixpoint eval_linsum_zsol ts zs :=
-  match ts with
-  | nil => Some 0%Z
-  | cons t ts' =>
-    match eval_linterm_zsol t zs with
-    | Some x =>
-      match eval_linsum_zsol ts' zs with
-      | Some r => Some (x + r)
-      | None => None
-      end
-    | None => None
-    end
-  end.
-
-Definition check_lincon_zsol lincon zs :=
-  match eval_linsum_zsol (fst lincon) zs with
-  | None => false
-  | Some k => Z_leb k (snd lincon)
-  end.
-
-Theorem eval_linterm_zsol_valid :
-  forall (zs : zsol) (v : Z) (theta : asg) (t : linterm),
-    eval_linterm_zsol t zs = Some v -> 
-      eval_zsol zs theta -> eval_linterm t theta = v.
-Proof.
-  intros.
-  unfold eval_linterm, eval_linterm_zsol in *; simpl.
-  remember (zsol_val zs (snd t)) as f; destruct f; destruct t; simpl in *.
-  apply eq_sym in Heqf; apply zsol_val_valid with (theta := theta) in Heqf; try assumption.
-  injection H; intros.
-  now rewrite Heqf.
-  discriminate.
-Qed.
-  
-Theorem eval_linsum_zsol_plus :
-  forall (zs : zsol) (v v' : Z) (a : linterm) (ts : list linterm),
-    eval_linterm_zsol a zs = Some v /\ eval_linsum_zsol ts zs = Some v' ->
-      eval_linsum_zsol (a :: ts) zs = Some (v + v').
-Proof.
-  intros.
-  unfold eval_linsum_zsol; fold eval_linsum_zsol.
-  remember (eval_linterm_zsol a zs) as ea; destruct ea.
-  remember (eval_linsum_zsol ts zs) as ets; destruct ets.
-  destruct H as [Hz Hz0]; inversion Hz; inversion Hz0.
-  trivial.
-  now destruct H. now destruct H.
-Qed.
-
-Fixpoint linsum_is_ground (zs : zsol) (ts : list linterm) :=
-  match ts with
-  | nil => True
-  | cons (_, x) ts' => ZMaps.In x zs /\ linsum_is_ground zs ts'
-  end.
-
-Theorem linsum_zsol_some_is_ground :
-  forall (zs : zsol) (ts : list linterm),
-    (exists k, eval_linsum_zsol ts zs = Some k) -> linsum_is_ground zs ts.
-Proof.
-  intros zs ts H.
-  induction ts; unfold eval_linsum_zsol, linsum_is_ground; simpl; try trivial.
-  eelim H; intro.
-  fold eval_linsum_zsol; fold eval_linsum; fold linsum_is_ground; destruct a; simpl.
-  intros; remember (eval_linterm_zsol (z, i) zs) as ez;
-    remember (eval_linsum_zsol ts zs) as ets.
-  destruct ez, ets; try congruence.
-  symmetry in Heqets, Heqez.
-  split.
-  unfold eval_linterm_zsol, zsol_val in Heqez; simpl in Heqez.
-  remember (ZMaps.find i zs) as fi; destruct fi; try congruence.
-  assert (ZMaps.In i zs \/ ~ ZMaps.In i zs).
-    tauto.
-  destruct H1; try assumption.
-  apply not_find_in_iff in H1. congruence.
-  apply IHts. eexists.
-  now instantiate (1 := z1).
-Qed.
-
-Theorem ground_linsum_eq :
-  forall (zs : zsol) (theta : asg) (ts : list linterm),
-    linsum_is_ground zs ts ->
-      eval_zsol zs theta -> eval_linsum_zsol ts zs = Some (eval_linsum ts theta).
-Proof.
-  intros zs theta ts.
-  induction ts.
-  unfold linsum_is_ground, eval_linsum_zsol, eval_linsum; tauto.
-  
-  unfold linsum_is_ground, eval_linsum_zsol, eval_linsum;
-    fold linsum_is_ground; fold eval_linsum_zsol; fold eval_linsum; intros.
-  destruct a; simpl in *. destruct H as [Hi Hg].
-  remember (eval_linterm_zsol (z, i) zs) as ea.
-  remember (eval_linsum_zsol ts zs) as ets.
-  apply IHts in Hg.
-  destruct ets; simpl in *.
-    inversion Hg as [Hz0]; clear Hg. rewrite <- Hz0.
-    destruct ea.
-    symmetry in Heqea; apply eval_linterm_zsol_valid with (theta := theta) in Heqea.
-    now rewrite Heqea. assumption.
-    unfold eval_linterm_zsol, zsol_val in Heqea; simpl in *.
-    remember (ZMaps.find i zs) as fi.
-    destruct fi; try discriminate.
-    symmetry in Heqfi; now apply not_find_in_iff in Heqfi.
-    discriminate. assumption.
-Qed.
-
-Theorem check_lincon_zsol_valid :
-    forall lincon zs,
-      (check_lincon_zsol lincon zs = true) ->
-        implies (eval_zsol zs) (eval_lincon lincon).
+Theorem check_lincon_sol_valid :
+    forall lincon theta,
+      (check_lincon_sol lincon theta = true) -> eval_lincon lincon theta.
 Proof.
   intros lincon zs; destruct lincon.
-  unfold check_lincon_zsol, implies; simpl.
-  remember (eval_linsum_zsol l zs) as el.
-  destruct el; symmetry in Heqel; try congruence.
-  assert (linsum_is_ground zs l).
-    apply linsum_zsol_some_is_ground; eexists; now instantiate (1 := z0).
-  unfold eval_lincon.
-  intros; simpl in *.
-  assert (eval_linsum_zsol l zs = Some (eval_linsum l theta)).
-    apply ground_linsum_eq; try assumption.
-  rewrite Heqel in H2.
-  inversion H2.
-  rewrite <- H4.
-  now apply Z_leb_iff_le in H0.
+  unfold check_lincon_sol;  simpl.
+  unfold eval_lincon; simpl.
+  intros; now apply Z_leb_iff_le.
 Qed.
 
-Definition LinearSolCheck := mkSolCheck LinearCon check_lincon_zsol check_lincon_zsol_valid.
+Definition LinearSolCheck := mkSolCheck LinearCon check_lincon_sol check_lincon_sol_valid.
